HOLean/Model.lean
@@ -3,3 +3,5 @@ import HOLean.Model.Basic
 import HOLean.Model.Ty
 import HOLean.Model.Const
 import HOLean.Model.Tm
+import HOLean.Model.Commute
+import HOLean.Model.Sound
